context_free_grammars/ContextFreeGrammarsProperties.fst
@@ -1,0 +1,2 @@
+module ContextFreeGrammarsProperties
+open ContextFreeGrammars
