context_free_grammars/ContextFreeGrammarsTests.fst
@@ -1,0 +1,2 @@
+module ContextFreeGrammarsTests
+open ContextFreeGrammars
